ADMIT intro_refine_slprop, intro_vrefine

pulse/ulib/experimental/Steel.SelEffect.fst
@@ -1001,3 +1001,5 @@ let write (#a:Type0) (r:ref a) (x:a) : SteelSel unit
     change_slprop (vptr r) (vptr_tmp r full_perm v) v () (elim_vptr r v);
     write0 v r x;
     change_slprop (vptr_tmp r full_perm x) (vptr r) () x (intro_vptr r x)
+
+let intro_vrefine v p = sladmit ()
